DynamoDbEncryption/dafny/DynamoDbItemEncryptor/src/AwsCryptographyDynamoDbEncryptionItemEncryptorOperations.dfy
@@ -488,26 +488,16 @@ module AwsCryptographyDynamoDbEncryptionItemEncryptorOperations refines Abstract
   }
 
   function method ConvertCryptoSchemaToAttributeActions(config: ValidConfig, schema: CSE.CryptoSchema)
-    : (ret: Result<map<ComAmazonawsDynamodbTypes.AttributeName, CSE.CryptoAction>, Error>)
-    ensures ret.Success? ==> forall k <- ret.value.Keys :: InSignatureScope(config, k)
-    ensures ret.Success? ==> forall k <- ret.value.Keys :: !ret.value[k].DO_NOTHING?
+    : (ret: map<ComAmazonawsDynamodbTypes.AttributeName, CSE.CryptoAction>)
+    requires schema.content.SchemaMap?;
+    requires forall k <- schema.content.SchemaMap :: schema.content.SchemaMap[k].content.Action?;
+    requires forall k <- schema.content.SchemaMap :: ComAmazonawsDynamodbTypes.IsValid_AttributeName(k);
+    requires forall k <- schema.content.SchemaMap :: !schema.content.SchemaMap[k].content.Action.DO_NOTHING?;
+    requires forall k <- schema.content.SchemaMap :: InSignatureScope(config, k);
+    ensures forall k <- ret.Keys :: InSignatureScope(config, k)
+    ensures forall k <- ret.Keys :: !ret[k].DO_NOTHING?
   {
-    // Any of these errors would indicate an internal error in our integration with the
-    // Structured Encryption Library. If we could thread through dafny verification
-    // at that integration, we would be able to ensure these properties.
-    // Because we are not modeled to trust that boundary, these must be runtime checks.
-    :- Need(schema.content.SchemaMap?,
-        DynamoDbItemEncryptorException( message := "Unexpected Crypto Schema in Parsed Header"));
-    var schemaMap := schema.content.SchemaMap;
-    :- Need(forall k <- schemaMap :: schemaMap[k].content.Action?,
-        DynamoDbItemEncryptorException( message := "Unexpected Crypto Schema in Parsed Header"));
-    :- Need(forall k <- schemaMap :: ComAmazonawsDynamodbTypes.IsValid_AttributeName(k),
-        DynamoDbItemEncryptorException( message := "Unexpected Crypto Schema in Parsed Header"));
-    :- Need(forall k <- schemaMap :: InSignatureScope(config, k),
-        DynamoDbItemEncryptorException( message := "Unexpected Crypto Schema in Parsed Header"));
-    :- Need(forall k <- schemaMap :: !schemaMap[k].content.Action.DO_NOTHING?,
-        DynamoDbItemEncryptorException( message := "Unexpected Crypto Schema in Parsed Header"));
-    Success(map k <- schema.content.SchemaMap.Keys | true :: k := schema.content.SchemaMap[k].content.Action)
+    map k <- schema.content.SchemaMap.Keys | true :: k := schema.content.SchemaMap[k].content.Action
   }
 
   predicate EncryptItemEnsuresPublicly(input: EncryptItemInput, output: Result<EncryptItemOutput, Error>)
@@ -579,7 +569,7 @@ module AwsCryptographyDynamoDbEncryptionItemEncryptorOperations refines Abstract
 
     //= specification/dynamodb-encryption-client/encrypt-item.md#behavior
     //= type=implication
-    //# If a [Plaintext Policy](./ddb-encryption-table-config.md#plaintext-policy) of
+    //# If a [Plaintext Policy](./ddb-table-encryption-config.md#plaintext-policy) of
     //# `REQUIRE_WRITE_ALLOW_READ` is specified,
     //# this operation MUST NOT encrypt the input item,
     //# and MUST passthrough that item as the output.
@@ -597,16 +587,16 @@ module AwsCryptographyDynamoDbEncryptionItemEncryptorOperations refines Abstract
     assert {:split_here} true;
 
     //= specification/dynamodb-encryption-client/encrypt-item.md#behavior
-    //# If a [Legacy Policy](./ddb-encryption-table-config.md#legacy-policy) of
+    //# If a [Legacy Policy](./ddb-table-encryption-config.md#legacy-policy) of
     //# `REQUIRE_ENCRYPT_ALLOW_DECRYPT` is specified,
     //# this operation MUST delegate encryption of this item to the
-    //# [Legacy Encryptor](./ddb-encryption-table-config.md#legacy-encryptor),
-    //# using the configured [Attribute Flags](./ddb-encryption-table-config.md) as input.
+    //# [Legacy Encryptor](./ddb-table-encryption-config.md#legacy-encryptor),
+    //# using the configured [Attribute Flags](./ddb-table-encryption-config.md) as input.
     if config.internalLegacyConfig.Some? && config.internalLegacyConfig.value.policy.REQUIRE_ENCRYPT_ALLOW_DECRYPT? {
       var encryptItemOutput :- config.internalLegacyConfig.value.EncryptItem(input);
       //= specification/dynamodb-encryption-client/encrypt-item.md#behavior
       //# The item returned by this operation MUST be the item outputted by the
-      //# [Legacy Encryptor](./ddb-encryption-table-config.md#legacy-encryptor).
+      //# [Legacy Encryptor](./ddb-table-encryption-config.md#legacy-encryptor).
       return Success(encryptItemOutput);
     }
 
@@ -677,7 +667,7 @@ module AwsCryptographyDynamoDbEncryptionItemEncryptorOperations refines Abstract
   {true}
 
   // public Decrypt method
-  method DecryptItem(config: InternalConfig, input: DecryptItemInput)
+  method {:vcs_split_on_every_assert} DecryptItem(config: InternalConfig, input: DecryptItemInput)
     returns (output: Result<DecryptItemOutput, Error>)
 
     //= specification/dynamodb-encryption-client/decrypt-item.md#dynamodb-item
@@ -755,10 +745,12 @@ module AwsCryptographyDynamoDbEncryptionItemEncryptorOperations refines Abstract
       //# data that was serialized into the header included in the output DynamoDb Item.
       && output.value.parsedHeader.Some?
       && var structuredEncParsed := Seq.Last(config.structuredEncryption.History.DecryptStructure).output.value.parsedHeader;
-      && var maybeParsedAuthAttrs := ConvertCryptoSchemaToAttributeActions(config, structuredEncParsed.cryptoSchema);
-      && maybeParsedAuthAttrs.Success?
+      && structuredEncParsed.cryptoSchema.content.SchemaMap?
+      && (forall k <- structuredEncParsed.cryptoSchema.content.SchemaMap :: structuredEncParsed.cryptoSchema.content.SchemaMap[k].content.Action? && !structuredEncParsed.cryptoSchema.content.SchemaMap[k].content.Action.DO_NOTHING?)
+      && (forall k <- structuredEncParsed.cryptoSchema.content.SchemaMap :: ComAmazonawsDynamodbTypes.IsValid_AttributeName(k))
+      && (forall k <- structuredEncParsed.cryptoSchema.content.SchemaMap :: InSignatureScope(config, k))
       && output.value.parsedHeader.value == ParsedHeader(
-          attributeActions := maybeParsedAuthAttrs.value,
+          attributeActions := ConvertCryptoSchemaToAttributeActions(config, structuredEncParsed.cryptoSchema),
           algorithmSuiteId := structuredEncParsed.algorithmSuiteId,
           storedEncryptionContext := structuredEncParsed.storedEncryptionContext,
           encryptedDataKeys := structuredEncParsed.encryptedDataKeys
@@ -766,7 +758,7 @@ module AwsCryptographyDynamoDbEncryptionItemEncryptorOperations refines Abstract
 
     //= specification/dynamodb-encryption-client/decrypt-item.md#behavior
     //= type=implication
-    //# If a [Plaintext Policy](./ddb-encryption-table-config.md#plaintext-policy) of
+    //# If a [Plaintext Policy](./ddb-table-encryption-config.md#plaintext-policy) of
     //# `REQUIRE_WRITE_ALLOW_READ` or `FORBID_WRITE_ALLOW_READ` is specified,
     //# and the input item [is a plaintext item](#determining-plaintext-items)
     //# this operation MUST NOT decrypt the input item,
@@ -785,25 +777,21 @@ module AwsCryptographyDynamoDbEncryptionItemEncryptorOperations refines Abstract
       && (config.sortKeyName.None? || config.sortKeyName.value in input.encryptedItem)
       , DynamoDbItemEncryptorException( message := "Configuration missmatch partition or sort key does not exist in item."));
 
-    assert {:split_here} true;
-
     //= specification/dynamodb-encryption-client/decrypt-item.md#behavior
-    //# If a [Legacy Policy](./ddb-encryption-table-config.md#legacy-policy) of
+    //# If a [Legacy Policy](./ddb-table-encryption-config.md#legacy-policy) of
     //# `REQUIRE_ENCRYPT_ALLOW_DECRYPT` or `FORBID_ENCRYPT_ALLOW_DECRYPT` is configured,
     //# and the input item [is an item written in the legacy format](#determining-legacy-items),
     //# this operation MUST delegate decryption of this item to the
-    //# [Legacy Encryptor](./ddb-encryption-table-config.md#legacy-encryptor),
-    //# using the configured [Attribute Flags](./ddb-encryption-table-config.md) as input.
+    //# [Legacy Encryptor](./ddb-table-encryption-config.md#legacy-encryptor),
+    //# using the configured [Attribute Flags](./ddb-table-encryption-config.md) as input.
     // Note: InternalLegacyConfig.DecryptItem checks that the legacy policy is correct.
     if config.internalLegacyConfig.Some? && config.internalLegacyConfig.value.IsLegacyInput(input) {
       var decryptItemOutput :- config.internalLegacyConfig.value.DecryptItem(input);
       //= specification/dynamodb-encryption-client/decrypt-item.md#behavior
       //# The item returned by this operation MUST be the item outputted by the
-      //# [Legacy Encryptor](./ddb-encryption-table-config.md#legacy-encryptor).
+      //# [Legacy Encryptor](./ddb-table-encryption-config.md#legacy-encryptor).
       return Success(decryptItemOutput);
     }
-
-    assert {:split_here} true;
 
     if (
       && (|| config.plaintextPolicy.REQUIRE_WRITE_ALLOW_READ?
@@ -830,8 +818,6 @@ module AwsCryptographyDynamoDbEncryptionItemEncryptorOperations refines Abstract
       content := CSE.StructuredDataContent.DataMap(encryptedStructure),
       attributes := None);
 
-    assert {:split_here} true;
-
     //= specification/dynamodb-encryption-client/decrypt-item.md#behavior
     //# This operation MUST create a
     //# [Required Encryption Context CMM](https://github.com/awslabs/private-aws-encryption-sdk-specification-staging/blob/dafny-verified/framework/required-encryption-context-cmm.md)
@@ -848,8 +834,6 @@ module AwsCryptographyDynamoDbEncryptionItemEncryptorOperations refines Abstract
     );
     var reqCMM :- reqCMMR.MapFailure(e => AwsCryptographyMaterialProviders(e));
 
-    assert {:split_here} true;
-
     var decryptRes := config.structuredEncryption.DecryptStructure(
       CSE.DecryptStructureInput(
         tableName := config.tableName,
@@ -862,15 +846,13 @@ module AwsCryptographyDynamoDbEncryptionItemEncryptorOperations refines Abstract
       )
     );
 
-    assert {:split_here} true;
-
     var decryptVal :- decryptRes.MapFailure(
         e => Error.AwsCryptographyDynamoDbEncryption(DDBE.AwsCryptographyStructuredEncryption(e)));
     var decryptedData := decryptVal.plaintextStructure;
     var ddbItem :- DynamoToStruct.StructuredToItem(decryptedData.content.DataMap)
         .MapFailure(e => Error.AwsCryptographyDynamoDbEncryption(e));
 
-    var parsedAuthActions :- ConvertCryptoSchemaToAttributeActions(config, decryptVal.parsedHeader.cryptoSchema);
+    var parsedAuthActions := ConvertCryptoSchemaToAttributeActions(config, decryptVal.parsedHeader.cryptoSchema);
 
     // Validate the parsed header is consistent with our signature scope configuration
 
