DynamoDbEncryption/dafny/DynamoDbItemEncryptor/Model/DynamoDbItemEncryptor.smithy
@@ -33,12 +33,12 @@ service DynamoDbItemEncryptor {
 //= type=implication
 //# On initialization of the DynamoDB Item Encryptor,
 //# the caller MUST provide all REQUIRED fields specified in
-//# [dynamodb encryption table config](./ddb-encryption-table-config.md).
+//# [dynamodb encryption table config](./ddb-table-encryption-config.md).
 
 //= specification/dynamodb-encryption-client/ddb-item-encryptor.md#initialization
 //= type=implication
 //# and the caller MAY provide any OPTIONAL field specified in
-//# [dynamodb encryption table config](./ddb-encryption-table-config.md).
+//# [dynamodb encryption table config](./ddb-table-encryption-config.md).
 
 structure DynamoDbItemEncryptorConfig {
     //= specification/dynamodb-encryption-client/ddb-table-encryption-config.md#structure
