specification/dynamodb-encryption-client/decrypt-item.md
@@ -74,22 +74,22 @@ representing the deserialized form of the header of the input encrypted structur
 
 ## Behavior
 
-If a [Legacy Policy](./ddb-encryption-table-config.md#legacy-policy) of
+If a [Legacy Policy](./ddb-table-encryption-config.md#legacy-policy) of
 `FORBID_ENCRYPT_FORBID_DECRYPT` is configured,
 and the input item [is an item written in the legacy format](#determining-legacy-items),
 this operation MUST fail.
 
-If a [Legacy Policy](./ddb-encryption-table-config.md#legacy-policy) of
+If a [Legacy Policy](./ddb-table-encryption-config.md#legacy-policy) of
 `REQUIRE_ENCRYPT_ALLOW_DECRYPT` or `FORBID_ENCRYPT_ALLOW_DECRYPT` is configured,
 and the input item [is an item written in the legacy format](#determining-legacy-items),
 this operation MUST delegate decryption of this item to the
-[Legacy Encryptor](./ddb-encryption-table-config.md#legacy-encryptor),
-using the configured [Attribute Flags](./ddb-encryption-table-config.md) as input.
+[Legacy Encryptor](./ddb-table-encryption-config.md#legacy-encryptor),
+using the configured [Attribute Flags](./ddb-table-encryption-config.md) as input.
 The item returned by this operation MUST be the item outputted by the
-[Legacy Encryptor](./ddb-encryption-table-config.md#legacy-encryptor).
+[Legacy Encryptor](./ddb-table-encryption-config.md#legacy-encryptor).
 Otherwise, this operations continues as follows.
 
-If a [Plaintext Policy](./ddb-encryption-table-config.md#plaintext-policy) of
+If a [Plaintext Policy](./ddb-table-encryption-config.md#plaintext-policy) of
 `REQUIRE_WRITE_ALLOW_READ` or `FORBID_WRITE_ALLOW_READ` is specified,
 and the input item [is a plaintext item](#determining-plaintext-items)
 this operation MUST NOT decrypt the input item,
